ironfleet/src/Dafny/Distributed/Concur/ReductionPlan.i.dfy
@@ -1,0 +1,35 @@
+include "Reduction.i.dfy"
+
+module ReductionPlanModule {
+
+    import opened ReductionModule
+
+    datatype ActorReductionPlan = ActorReductionPlan(ab:seq<ActorState>, trees:seq<Tree>)
+    type ReductionPlan = map<Actor, ActorReductionPlan>
+
+    predicate IsValidActorReductionPlan(plan:ActorReductionPlan)
+    {
+           |plan.ab| == |plan.trees| + 1
+        && (forall tree :: tree in plan.trees ==> TreeValid(tree))
+    }
+
+    predicate IsValidReductionPlan(config:Config, plan:ReductionPlan)
+    {
+            NoActor() !in config.tracked_actors
+         && (forall actor :: actor in config.tracked_actors ==> actor in plan && IsValidActorReductionPlan(plan[actor]))
+    }
+
+    function RestrictTraceToTrackedActions(trace:Trace) : Trace
+        ensures var trace':= RestrictTraceToTrackedActions(trace);
+                forall entry {:trigger entry in trace'}{:trigger IsTrackedAction(entry.action)} ::
+                         entry in trace' ==> IsTrackedAction(entry.action);
+    {
+        if trace == [] then
+            []
+        else if IsTrackedAction(trace[0].action) then
+            [trace[0]] + RestrictTraceToTrackedActions(trace[1..])
+        else
+            RestrictTraceToTrackedActions(trace[1..])
+    }
+
+}
