ironfleet/src/Dafny/Distributed/Concur/UltimateReduction.i.dfy
@@ -1,0 +1,24 @@
+include "RemoveUpdates.i.dfy"
+include "SpecRefinement.i.dfy"
+include "ReductionPlan.i.dfy"
+
+module UltimateReductionModule {
+
+    import opened RemoveUpdatesModule
+    import opened SpecRefinementModule
+    import opened ReductionPlanModule
+
+    lemma lemma_UltimateReduction(
+        config:Config,
+        trace:Trace,
+        lb:SystemBehavior,
+        plan:ReductionPlan
+        )
+        requires IsValidSystemTraceAndBehavior(config, trace, lb);
+        requires IsValidReductionPlan(config, plan);
+        requires forall actor :: actor in config.tracked_actors ==>
+                     RestrictTraceToTrackedActions(RestrictTraceToActor(trace, actor)) == GetEntries(plan[actor].trees);
+        ensures  SystemBehaviorRefinesSpec(lb);
+
+}
+
