ironfleet/src/Dafny/Distributed/Concur/UltimateRefinement.i.dfy
@@ -5,10 +5,11 @@ module UltimateRefinementModule {
     import opened SpecRefinementModule
 
     lemma {:axiom} lemma_UltimateRefinement(
+        config:Config,
         trace:Trace,
         lb:SystemBehavior
         )
-        requires IsValidSystemTraceAndBehavior(trace, lb);
+        requires IsValidSystemTraceAndBehavior(config, trace, lb);
         requires forall entry :: entry in trace ==>
                             if entry.actor in lb[0].config.tracked_actors then entry.action.HostNext? else IsRealAction(entry.action);
         ensures  SystemBehaviorRefinesSpec(lb);
